shift-reset/core/kont.v
@@ -9,8 +9,8 @@ Fixpoint kont_append (k1 k2 : kont) : kont :=
 Definition metakont_extend (mk : metakont) (k : kont) : metakont :=
   match mk with
   | MKPure k' => MKPure (kont_append k' k)
-  | MKReset mk' k' => MKReset mk' (kont_append k' k)
-  | MKPrompt mk' k' => MKPrompt mk' (kont_append k' k)
+  | MKReset mk' tag k' => MKReset mk' tag (kont_append k' k)
+  | MKPrompt mk' tag k' => MKPrompt mk' tag (kont_append k' k)
   | MKTry mk' c k' => MKTry mk' c (kont_append k' k)
   | MKHandle mk' c k' => MKHandle mk' c (kont_append k' k)
   | MKShallowHandle mk' c k' => MKShallowHandle mk' c (kont_append k' k)
