shift-reset/core/tag.v
@@ -4,3 +4,5 @@ Record tag : Type := Tag { tag_car : string }.
 
 Definition tag_eq_dec : forall (tag1 tag2 : tag), {tag1 = tag2} + {tag1 <> tag2}.
 Proof. decide equality; auto using string_dec. Defined.
+
+Definition tag_empty : tag := Tag "".
